1.
	a. Everything is a square + 1 so we have $a_n = n^2 + 1$

	b. This looks like triangular numbers - 1 so $a_n = \dfrac{n(n+1)}{2} - 1$

	c. These are triangular numbers +2 starting at 6, so its $a_n = \dfrac{(n+2)(n+3)}{2} + 2$

	d. Its factorials - 1 and seemingly starting at 2. $a_n = (n+1)-1$ 
2.
	a. This is a tough one. The between numbers doubles everytime, but writing this out would be recursive. The difference between triangular numbers also doubles everytime. Its just triangles numbers + 4 so $\dfrac{n(n+1)}{2} + 4$
	
	b. The differences are 3, 5, 7, 9, 11, they start at 3 and increase by 2 everytime. We this same pattern in in square numbers so this one is but this one is one position left and down one. So its $a_n = (n + 1)^2 - 1$.

	c. Once again the difference is increasing by 2 every time, so I recognize this as some sort of square number sequence. I think it is $(n+3)^2 - 3 - 1n$

	d. Very confusing. No discernable patter in the plain numbers or the difference between them. I will come back to this.
3.
	a. 0, 1, 3, 6, 10. $a_n = a_n-1 + n$ given $a_0 = 0$
	b. 0, 1, 2, 3, 4. $a_n = n$
	c. 1, 1, 2, 6, 24. $a_n = n!$
